
\begin{lemma}[Segre's lemma of tangents, simplified version]

\end{lemma}

\begin{proof}
    The (probably) simplest proof is by induction on $\card{\cA}$.
    for $\card\cA=n-1$ choose $b\in \field{q}^n\setminus\gen\cA$ and define
    $$
    T_A:=\prod_{\lambda\in\field{q}}{(\dual{a}+\lambda\dual{b})}
    $$
    where $\set{a}=\cA\setminus A$ and $\dual b, \dual a$ mean elements from the dual basis of $\cA\setjoin\set{b}$. For $x_1,x_2,X$ we get that
    $$
    T_{X\setjoin\set{x_1}}(x_2)=1=T_{X\setjoin\set{x_2}}(x_1)
    $$
    as desired.
        For the induction step assume that $\card{\cA}\geq n$. Set $a:=\min{\cA}$ and define the tangent polynomials $T^{\cA}_Y$ via the tangent polynomials $T^{\cA'}_{Y'}$ ($\cA':=\cA\setminus\set{a}$, $Y\setleq\cA$, $Y'\setleq\cA'$, $\card{Y}=\card{Y'}=n-2$) by
        $$
        T^{\cA}_{Y'}:=\frac{T^{\cA'}_{Y'}}{\det(a,Y',\arg)}
        $$
        and
        $$
        T^{\cA}_{X'\setjoin\set{a}}:=\prod
        $$
        (this is a definition since the symmetric algebra is a UFD).
\end{proof}